Fix quotation after primitive array support

quotation/theories/ToPCUIC/PCUIC/utils/PCUICPrimitive.v
@@ -1,12 +1,87 @@
+From MetaCoq.Utils.MCTactics Require Import DestructHead UniquePose.
 From MetaCoq.PCUIC Require Import utils.PCUICPrimitive.
 From MetaCoq.Quotation.ToPCUIC Require Import Init.
 From MetaCoq.Quotation.ToPCUIC Require Import (hints) Coq.Init Coq.Numbers Coq.Floats.
 From MetaCoq.Quotation.ToPCUIC.Common Require Import (hints) Universes Primitive.
+From MetaCoq.Quotation.ToPCUIC.Utils Require Import (hints) All_Forall.
 
 #[export] Instance quote_array_model {term} {qterm : quotation_of term} {quote_term : ground_quotable term} : ground_quotable (array_model term) := ltac:(destruct 1; exact _).
+
+#[export] Instance quotation_of_array_model {term a} {qterm : quotation_of term} {qa : @tPrimProp term quotation_of (existT _ Primitive.primArray (primArrayModel a))} : quotation_of a
+  := ltac:(cbv -[quotation_of] in qa; destruct a; destruct_head'_prod; exact _).
+
+#[export] Hint Extern 0 (@tPrimProp ?term quotation_of ?a)
+=> lazymatch goal with
+   | [ H : @tPrimProp _ quotation_of _ |- _ ] => assumption
+   end : typeclass_instances.
 
 #[export] Instance quote_prim_model {term tag} {qterm : quotation_of term} {quote_term : ground_quotable term} : ground_quotable (prim_model term tag) := ltac:(destruct 1; eauto).
 
 #[export] Instance quote_prim_model_of {term tag} {qterm : quotation_of term} {quote_term : ground_quotable term} : ground_quotable (prim_model_of term tag) := ltac:(cbv [prim_model_of]; destruct tag; exact _).
 
 #[export] Instance quote_prim_val {term} {qterm : quotation_of term} {quote_term : ground_quotable term} : ground_quotable (prim_val term) := ltac:(cbv [prim_val]; exact _).
+
+#[export] Instance quotation_of_prim_val {term} {p : prim_val term} {qterm : quotation_of term} {qp : @tPrimProp term quotation_of p} : quotation_of p := ltac:(destruct p as [? p]; destruct p; exact _).
+
+Definition quote_onPrims {term eq_term leq_term u u'} {qterm : quotation_of term} {qeq_term : quotation_of eq_term} {qleq_term : quotation_of leq_term}
+  {quote_term : ground_quotable term}
+  {quote_eq_term : forall x y, ground_quotable (eq_term x y)}
+  {quote_leq_term : forall x y, ground_quotable (leq_term x y)} : ground_quotable (@onPrims term eq_term leq_term u u')
+  := ltac:(destruct 1; exact _).
+
+Definition quote_onPrims_Type_Prop {term eq_term} {leq_term : _ -> _ -> Prop} {u u'} {qterm : quotation_of term} {qeq_term : quotation_of eq_term} {qleq_term : quotation_of leq_term}
+  {quote_term : ground_quotable term}
+  {quote_eq_term : forall x y, ground_quotable (eq_term x y)}
+  {quote_leq_term : forall x y, ground_quotable (leq_term x y)} : ground_quotable (@onPrims term eq_term leq_term u u')
+  := @quote_onPrims term eq_term leq_term u u' qterm qeq_term qleq_term quote_term quote_eq_term quote_leq_term.
+
+Definition quote_onPrims_via_dep
+  {term eq_term leq_term u u' p} {eq_term_dep leq_term_dep}
+  {qp : @onPrims_dep term eq_term leq_term eq_term_dep leq_term_dep u u' p}
+  {qterm : quotation_of term} {qeq_term : quotation_of eq_term} {qleq_term : quotation_of leq_term}
+  {quote_term : ground_quotable term}
+  {quote_eq_term : forall x y e, eq_term_dep x y e -> quotation_of e}
+  {quote_leq_term : forall x y e, leq_term_dep x y e -> quotation_of e}
+  : quotation_of p.
+Proof.
+  destruct qp.
+  all: lazymatch goal with
+       | [ H : All_Forall.All2_dep ?T ?x |- _ ]
+         => lazymatch T with
+            | (fun _ _ r => quotation_of r) => idtac
+            | _
+              => assert (All_Forall.All2_dep (fun _ _ r => quotation_of r) x);
+                 [ eapply All_Forall.All2_dep_impl; try exact H; [];
+                   cbv beta; intros;
+                   repeat match goal with
+                     | [ H : _ * _ |- _ ] => destruct H
+                     end;
+                   cbn [fst snd] in *
+                 | clear H ]
+            end
+       | _ => idtac
+       end.
+  all: repeat (let H := multimatch goal with H : _ |- _ => H end in
+               first [ unique pose proof (quote_leq_term _ _ _ H)
+                     | unique pose proof (quote_eq_term _ _ _ H) ]).
+  all: exact _.
+Defined.
+
+#[export] Hint Extern 0 (@quotation_of (@onPrims ?term ?eq_term ?leq_term ?u ?u') ?x)
+=> lazymatch goal with
+   | [ H : @onPrims_dep _ _ _ ?eq_term_dep ?leq_term_dep _ _ x |- _ ]
+     => simple apply (@quote_onPrims_via_dep term eq_term leq_term u u' x eq_term_dep leq_term_dep H)
+   | _ => simple apply @quote_ground;
+          tryif (lazymatch type of leq_term with
+                 | _ -> _ -> Prop => idtac
+                 | Relation_Definitions.relation _ => idtac
+                 end)
+          then simple apply (@quote_onPrims_Type_Prop term eq_term leq_term u u')
+          else simple apply (@quote_onPrims term eq_term leq_term u u')
+   end
+  : typeclass_instances.
+#[export] Hint Cut [
+    ( _ * )
+      quote_ground
+      quote_onPrims
+  ] : typeclass_instances.
